Test/datatypes/runtest.bat
@@ -4,7 +4,7 @@ setlocal
 set BOOGIEDIR=..\..\Binaries
 set BPLEXE=%BOOGIEDIR%\Boogie.exe
 
-for %%f in (t1.bpl) do (
+for %%f in (t1.bpl t2.bpl) do (
   echo.
   echo -------------------- %%f --------------------
   %BPLEXE% %* /typeEncoding:m %%f
